[utils] Add lemmas for arrays

src/Utils.v
@@ -1,6 +1,7 @@
 (*! Useful definitions !*)
 From Coq Require Import Lists.List ZArith NArith.
 From PresburgerAI Require Import EqDec.
+Require Import Coq.Logic.ProofIrrelevance.
 
 (** Nonnegative integers less than n **)
 Definition Fin (n: nat) := { v : nat | v < n}.
@@ -8,16 +9,18 @@ Definition Fin (n: nat) := { v : nat | v < n}.
 (** List with fixed size **)
 Definition Array (T: Type) (n: nat) := { l : list T | length l = n }.
 
-(** Access the array at a given index **)
-Definition array_get {T: Type} {n: nat} (a: Array T n) (i: Fin n) : T.
-  destruct a.
+Definition get_default {T: Type} {n: nat} (a: Array T n) (i: Fin n) : T.
   destruct i.
-  subst.
-  apply nth_error_Some in l.
-  destruct (nth_error x x0).
-  - apply t.
-  - destruct l. reflexivity.
+  destruct a.
+  destruct n; intuition.
+  destruct x0; intuition.
+  simpl in e.
+  inversion e.
 Defined.
+
+(** Access the array at a given index **)
+Definition array_get {T: Type} {n: nat} (a: Array T n) (i: Fin n) :=
+  nth (proj1_sig i) (proj1_sig a) (get_default a i).
 
 Fixpoint set_nth {T: Type} (l: list T) (n: nat) (t: T) :=
   match l with
@@ -39,18 +42,71 @@ Proof.
 Qed.
 
 Lemma nth_set_nth :
-  forall (n: nat) {T: Type} (l: list T),
-  n < length l ->
-  forall t, nth_error (set_nth l n t) n = Some t.
+  forall {T: Type} (l: list T) (n1 n2: nat),
+    n1 < length l ->
+    n2 < length l ->
+    forall t, nth_error (set_nth l n1 t) n2 =
+         if n1 == n2 then
+           Some t
+         else
+           nth_error l n2.
 Proof.
-  induction n; intros; destruct l; simpl in *; intuition.
+  induction l; [intros; simpl in *; intuition | ].
+  simpl in *.
+  destruct n1; [ destruct n2; auto | ].
+  - destruct n2; intuition.
+    simpl in *.
+    apply lt_S_n in H.
+    apply lt_S_n in H0.
+    rewrite IHl; auto.
+    destruct (n1 == n2).
+    + cbv in e. subst.
+      destruct (S n2 == S n2); intuition.
+    + destruct (S n1 == S n2); intuition.
+      inversion e.
+      subst. intuition.
 Qed.
 
 (** Set the value on an index **)
 Definition array_set {T: Type} {n: nat} (a: Array T n) (i: Fin n) (t: T) : Array T n.
-  destruct a.
-  destruct i.
-  subst.
   eapply exist.
-  apply (set_nth_length x0 x t).
+  unfold Array in a.
+  rewrite <-(proj2_sig a) at 1.
+  apply (set_nth_length (proj1_sig i) (proj1_sig a) t).
 Defined.
+
+
+Lemma array_get_set_eq {T: Type} {n: nat} (a: Array T n) (i: Fin n) (t: T) :
+  array_get (array_set a i t) i = t.
+Proof.
+  unfold array_get, array_set.
+  simpl.
+  apply nth_error_nth.
+  destruct a, i.
+  simpl in *; subst.
+  rewrite nth_set_nth; intuition.
+  pose proof (equiv_dec_refl x0) as [? ?].
+  rewrite H; auto.
+Qed.
+
+
+Lemma array_get_set_ne {T: Type} {n: nat} (a: Array T n) (i1 i2: Fin n) (t: T) :
+  i1 <> i2 ->
+  array_get (array_set a i1 t) i2 = array_get a i2.
+Proof.
+  unfold array_get, array_set.
+  simpl.
+  intros.
+  apply nth_error_nth.
+  destruct a. simpl.
+  destruct i1, i2. subst.
+  simpl (proj1_sig _).
+  rewrite nth_set_nth; intuition.
+  destruct (equiv_dec x0 x1).
+  - destruct e.
+    exfalso.
+    apply H.
+    f_equal.
+    apply proof_irrelevance.
+  - auto using nth_error_nth'.
+Qed.
